src/ocaml-output/FStar_TypeChecker_Positivity.ml
@@ -1,4 +1,18 @@
 open Prims
+let (normalize :
+  FStar_TypeChecker_Env.env ->
+    FStar_Syntax_Syntax.term -> FStar_Syntax_Syntax.term)
+  =
+  fun env ->
+    fun t ->
+      FStar_TypeChecker_Normalize.normalize
+        [FStar_TypeChecker_Env.Beta;
+        FStar_TypeChecker_Env.HNF;
+        FStar_TypeChecker_Env.Weak;
+        FStar_TypeChecker_Env.Iota;
+        FStar_TypeChecker_Env.Exclude FStar_TypeChecker_Env.Zeta;
+        FStar_TypeChecker_Env.UnfoldUntil FStar_Syntax_Syntax.delta_constant]
+        env t
 let (debug_positivity :
   FStar_TypeChecker_Env.env_t -> (unit -> Prims.string) -> unit) =
   fun env ->
@@ -136,15 +150,7 @@ let rec (ty_strictly_positive_in_type :
               (fun uu___1 ->
                  let uu___2 = FStar_Syntax_Print.term_to_string in_type in
                  Prims.op_Hat "Checking strict positivity in type: " uu___2);
-            (let in_type1 =
-               FStar_TypeChecker_Normalize.normalize
-                 [FStar_TypeChecker_Env.Beta;
-                 FStar_TypeChecker_Env.HNF;
-                 FStar_TypeChecker_Env.Weak;
-                 FStar_TypeChecker_Env.Iota;
-                 FStar_TypeChecker_Env.Exclude FStar_TypeChecker_Env.Zeta;
-                 FStar_TypeChecker_Env.UnfoldUntil
-                   FStar_Syntax_Syntax.delta_constant] env in_type in
+            (let in_type1 = normalize env in_type in
              debug_positivity env
                (fun uu___2 ->
                   let uu___3 = FStar_Syntax_Print.term_to_string in_type1 in
@@ -477,23 +483,29 @@ and (ty_strictly_positive_in_arguments_to_fvar :
                      FStar_Compiler_Util.format3
                        "Checking positivity of %s in application of fv %s to %s"
                        uu___2 uu___3 uu___4);
-                (let uu___1 = FStar_TypeChecker_Env.datacons_of_typ env fv in
+                (let fv_ty =
+                   let uu___1 = FStar_TypeChecker_Env.try_lookup_lid env fv in
+                   match uu___1 with
+                   | FStar_Pervasives_Native.Some ((uu___2, fv_ty1), uu___3)
+                       -> fv_ty1
+                   | uu___2 ->
+                       let uu___3 =
+                         let uu___4 =
+                           let uu___5 = FStar_Ident.string_of_lid fv in
+                           FStar_Compiler_Util.format1
+                             "Type of %s not found when checking positivity"
+                             uu___5 in
+                         (FStar_Errors.Error_InductiveTypeNotSatisfyPositivityCondition,
+                           uu___4) in
+                       let uu___4 = FStar_Ident.range_of_lid fv in
+                       FStar_Errors.raise_error uu___3 uu___4 in
+                 let uu___1 = FStar_TypeChecker_Env.datacons_of_typ env fv in
                  match uu___1 with
                  | (b, idatas) ->
                      if Prims.op_Negation b
                      then
-                       let uu___2 =
-                         FStar_TypeChecker_Env.try_lookup_lid env fv in
-                       (match uu___2 with
-                        | FStar_Pervasives_Native.Some
-                            ((uu___3, fv_ty), uu___4) ->
-                            check_ty_strictly_positive_in_args env mutuals
-                              ty_lid fv_ty args unfolded
-                        | FStar_Pervasives_Native.None ->
-                            (debug_positivity env
-                               (fun uu___4 ->
-                                  "Checking positivity of an application, head type not found, return false");
-                             false))
+                       check_ty_strictly_positive_in_args env mutuals ty_lid
+                         fv_ty args unfolded
                      else
                        (let ilid = fv in
                         let uu___3 = already_unfolded ilid args unfolded env in
@@ -504,35 +516,147 @@ and (ty_strictly_positive_in_arguments_to_fvar :
                                 "Checking nested positivity, we have already unfolded this inductive with these args");
                            true)
                         else
-                          (let num_ibs =
+                          (let num_params =
                              let uu___5 =
                                FStar_TypeChecker_Env.num_inductive_ty_params
                                  env ilid in
                              FStar_Compiler_Option.get uu___5 in
-                           let params =
-                             let uu___5 =
-                               FStar_Compiler_List.splitAt num_ibs args in
-                             FStar_Pervasives_Native.fst uu___5 in
-                           debug_positivity env
-                             (fun uu___6 ->
-                                let uu___7 = FStar_Ident.string_of_lid ilid in
-                                let uu___8 =
-                                  FStar_Syntax_Print.args_to_string params in
-                                FStar_Compiler_Util.format3
-                                  "Checking positivity in datacon, number of type parameters is %s, adding %s to the memo table"
-                                  (Prims.string_of_int num_ibs) uu___7 uu___8);
-                           (let uu___7 =
-                              let uu___8 =
-                                FStar_Compiler_Effect.op_Bang unfolded in
-                              FStar_List_Tot_Base.op_At uu___8
-                                [(ilid, params, num_ibs)] in
-                            FStar_Compiler_Effect.op_Colon_Equals unfolded
-                              uu___7);
-                           FStar_Compiler_List.for_all
-                             (fun d ->
-                                ty_strictly_positive_in_datacon_of_applied_inductive
-                                  env mutuals ty_lid d ilid us args num_ibs
-                                  unfolded) idatas)))
+                           let uu___5 =
+                             FStar_Compiler_List.splitAt num_params args in
+                           match uu___5 with
+                           | (params, indexes) ->
+                               let uu___6 =
+                                 FStar_Syntax_Util.arrow_formals fv_ty in
+                               (match uu___6 with
+                                | (fv_formals, uu___7) ->
+                                    (if
+                                       num_params >
+                                         (FStar_Compiler_List.length
+                                            fv_formals)
+                                     then
+                                       (let uu___9 =
+                                          let uu___10 =
+                                            let uu___11 =
+                                              FStar_Ident.string_of_lid fv in
+                                            let uu___12 =
+                                              FStar_Syntax_Print.term_to_string
+                                                fv_ty in
+                                            FStar_Compiler_Util.format4
+                                              "Expected a type with %s parameters, but %s : %s has only %s parameters"
+                                              (Prims.string_of_int num_params)
+                                              uu___11 uu___12
+                                              (Prims.string_of_int
+                                                 (FStar_Compiler_List.length
+                                                    fv_formals)) in
+                                          (FStar_Errors.Error_InductiveTypeNotSatisfyPositivityCondition,
+                                            uu___10) in
+                                        let uu___10 =
+                                          FStar_Ident.range_of_lid fv in
+                                        FStar_Errors.raise_error uu___9
+                                          uu___10)
+                                     else ();
+                                     (let fv_params =
+                                        let uu___9 =
+                                          FStar_Compiler_List.splitAt
+                                            num_params fv_formals in
+                                        FStar_Pervasives_Native.fst uu___9 in
+                                      let rec prefix_of_uniform_params
+                                        uniform_params params1 formals =
+                                        match (params1, formals) with
+                                        | ([], []) ->
+                                            ((FStar_Compiler_List.rev
+                                                uniform_params), [])
+                                        | (p::params2, f::formals1) ->
+                                            let uu___9 =
+                                              FStar_Syntax_Util.has_attribute
+                                                f.FStar_Syntax_Syntax.binder_attrs
+                                                FStar_Parser_Const.binder_non_uniformly_recursive_parameter_attr in
+                                            if uu___9
+                                            then
+                                              ((FStar_Compiler_List.rev
+                                                  uniform_params), (p ::
+                                                params2))
+                                            else
+                                              prefix_of_uniform_params (p ::
+                                                uniform_params) params2
+                                                formals1
+                                        | uu___9 ->
+                                            failwith
+                                              "impossible: they have the same length" in
+                                      let uu___9 =
+                                        prefix_of_uniform_params [] params
+                                          fv_params in
+                                      match uu___9 with
+                                      | (params1, non_uniform_params) ->
+                                          let indexes1 =
+                                            FStar_List_Tot_Base.op_At
+                                              non_uniform_params indexes in
+                                          (FStar_Compiler_List.iter
+                                             (fun uu___11 ->
+                                                match uu___11 with
+                                                | (index, uu___12) ->
+                                                    let uu___13 =
+                                                      FStar_Compiler_List.tryFind
+                                                        (fun mutual ->
+                                                           ty_occurs_in
+                                                             mutual index)
+                                                        (ty_lid :: mutuals) in
+                                                    (match uu___13 with
+                                                     | FStar_Pervasives_Native.Some
+                                                         mutual ->
+                                                         let uu___14 =
+                                                           let uu___15 =
+                                                             let uu___16 =
+                                                               FStar_Ident.string_of_lid
+                                                                 mutual in
+                                                             let uu___17 =
+                                                               FStar_Ident.string_of_lid
+                                                                 fv in
+                                                             FStar_Compiler_Util.format2
+                                                               "Type %s is not striclty positive since it instantiates a non-uniformly recursive parameter or index of %s"
+                                                               uu___16
+                                                               uu___17 in
+                                                           (FStar_Errors.Error_InductiveTypeNotSatisfyPositivityCondition,
+                                                             uu___15) in
+                                                         let uu___15 =
+                                                           FStar_Ident.range_of_lid
+                                                             fv in
+                                                         FStar_Errors.raise_error
+                                                           uu___14 uu___15
+                                                     | uu___14 -> ()))
+                                             indexes1;
+                                           (let num_uniform_params =
+                                              FStar_Compiler_List.length
+                                                params1 in
+                                            debug_positivity env
+                                              (fun uu___12 ->
+                                                 let uu___13 =
+                                                   FStar_Ident.string_of_lid
+                                                     ilid in
+                                                 let uu___14 =
+                                                   FStar_Syntax_Print.args_to_string
+                                                     params1 in
+                                                 FStar_Compiler_Util.format3
+                                                   "Checking positivity in datacon, number of type parameters is %s, adding %s %s to the memo table"
+                                                   (Prims.string_of_int
+                                                      num_uniform_params)
+                                                   uu___13 uu___14);
+                                            (let uu___13 =
+                                               let uu___14 =
+                                                 FStar_Compiler_Effect.op_Bang
+                                                   unfolded in
+                                               FStar_List_Tot_Base.op_At
+                                                 uu___14
+                                                 [(ilid, params1,
+                                                    num_uniform_params)] in
+                                             FStar_Compiler_Effect.op_Colon_Equals
+                                               unfolded uu___13);
+                                            FStar_Compiler_List.for_all
+                                              (fun d ->
+                                                 ty_strictly_positive_in_datacon_of_applied_inductive
+                                                   env mutuals ty_lid d ilid
+                                                   us args num_uniform_params
+                                                   unfolded) idatas))))))))
 and (ty_strictly_positive_in_datacon_of_applied_inductive :
   FStar_TypeChecker_Env.env_t ->
     FStar_Ident.lident Prims.list ->
@@ -643,6 +767,129 @@ let (name_strictly_positive_in_type :
         let t1 = FStar_Syntax_Subst.subst [FStar_Syntax_Syntax.NT (bv, fv)] t in
         let uu___ = FStar_Compiler_Util.mk_ref [] in
         ty_strictly_positive_in_type env [] fv_lid t1 uu___
+let (no_constructed_occurrences :
+  FStar_TypeChecker_Env.env_t ->
+    FStar_Syntax_Syntax.bv -> FStar_Syntax_Syntax.term -> Prims.bool)
+  =
+  fun env ->
+    fun var ->
+      fun ty ->
+        let uu___ =
+          let uu___1 = FStar_Syntax_Free.names ty in
+          FStar_Compiler_Util.set_mem var uu___1 in
+        if uu___
+        then
+          let uu___1 =
+            let uu___2 = FStar_Syntax_Subst.compress ty in
+            uu___2.FStar_Syntax_Syntax.n in
+          match uu___1 with
+          | FStar_Syntax_Syntax.Tm_name uu___2 -> true
+          | uu___2 -> false
+        else true
+let (check_parameter_is_recursively_uniform_in_type :
+  FStar_TypeChecker_Env.env_t ->
+    FStar_Ident.lident Prims.list ->
+      FStar_Syntax_Syntax.bv -> FStar_Syntax_Syntax.term -> Prims.bool)
+  =
+  fun env ->
+    fun mutuals ->
+      fun var ->
+        fun ty ->
+          let ty1 = normalize env ty in
+          let rec aux ty2 =
+            debug_positivity env
+              (fun uu___1 ->
+                 let uu___2 = FStar_Syntax_Print.bv_to_string var in
+                 let uu___3 = FStar_Syntax_Print.term_to_string ty2 in
+                 FStar_Compiler_Util.format2 "Recursively uniform? %s in %s"
+                   uu___2 uu___3);
+            (let uu___1 =
+               let uu___2 = FStar_Syntax_Subst.compress ty2 in
+               uu___2.FStar_Syntax_Syntax.n in
+             match uu___1 with
+             | FStar_Syntax_Syntax.Tm_name uu___2 -> true
+             | FStar_Syntax_Syntax.Tm_fvar uu___2 -> true
+             | FStar_Syntax_Syntax.Tm_uinst uu___2 -> true
+             | FStar_Syntax_Syntax.Tm_type uu___2 -> true
+             | FStar_Syntax_Syntax.Tm_constant uu___2 -> true
+             | FStar_Syntax_Syntax.Tm_refine (x, f) ->
+                 let uu___2 = aux x.FStar_Syntax_Syntax.sort in
+                 if uu___2
+                 then
+                   let uu___3 =
+                     let uu___4 =
+                       let uu___5 = FStar_Syntax_Syntax.mk_binder x in
+                       [uu___5] in
+                     FStar_Syntax_Subst.open_term uu___4 f in
+                   (match uu___3 with | (uu___4, f1) -> aux f1)
+                 else false
+             | FStar_Syntax_Syntax.Tm_app uu___2 ->
+                 let uu___3 = FStar_Syntax_Util.head_and_args ty2 in
+                 (match uu___3 with
+                  | (head, args) ->
+                      let uu___4 =
+                        let uu___5 = FStar_Syntax_Util.un_uinst head in
+                        uu___5.FStar_Syntax_Syntax.n in
+                      (match uu___4 with
+                       | FStar_Syntax_Syntax.Tm_fvar fv ->
+                           let uu___5 =
+                             FStar_Compiler_List.existsML
+                               (FStar_Syntax_Syntax.fv_eq_lid fv) mutuals in
+                           if uu___5
+                           then
+                             FStar_Compiler_List.for_all
+                               (fun uu___6 ->
+                                  match uu___6 with
+                                  | (arg, uu___7) ->
+                                      no_constructed_occurrences env var arg)
+                               args
+                           else
+                             FStar_Compiler_List.for_all
+                               (fun uu___7 ->
+                                  match uu___7 with
+                                  | (arg, uu___8) -> aux arg) args
+                       | uu___5 ->
+                           (aux head) &&
+                             (FStar_Compiler_List.for_all
+                                (fun uu___6 ->
+                                   match uu___6 with
+                                   | (arg, uu___7) -> aux arg) args)))
+             | FStar_Syntax_Syntax.Tm_abs uu___2 ->
+                 let uu___3 = FStar_Syntax_Util.abs_formals ty2 in
+                 (match uu___3 with
+                  | (bs, body, uu___4) ->
+                      (FStar_Compiler_List.for_all
+                         (fun b ->
+                            aux
+                              (b.FStar_Syntax_Syntax.binder_bv).FStar_Syntax_Syntax.sort)
+                         bs)
+                        && (aux body))
+             | FStar_Syntax_Syntax.Tm_arrow uu___2 ->
+                 let uu___3 = FStar_Syntax_Util.arrow_formals ty2 in
+                 (match uu___3 with
+                  | (bs, r) ->
+                      (FStar_Compiler_List.for_all
+                         (fun b ->
+                            aux
+                              (b.FStar_Syntax_Syntax.binder_bv).FStar_Syntax_Syntax.sort)
+                         bs)
+                        && (aux r))
+             | FStar_Syntax_Syntax.Tm_match
+                 (scrutinee, uu___2, branches, uu___3) ->
+                 (aux scrutinee) &&
+                   (FStar_Compiler_List.for_all
+                      (fun uu___4 ->
+                         match uu___4 with
+                         | (p, uu___5, t) ->
+                             let bs =
+                               let uu___6 = FStar_Syntax_Syntax.pat_bvs p in
+                               FStar_Compiler_List.map
+                                 FStar_Syntax_Syntax.mk_binder uu___6 in
+                             let uu___6 = FStar_Syntax_Subst.open_term bs t in
+                             (match uu___6 with | (bs1, t1) -> aux t1))
+                      branches)
+             | uu___2 -> false) in
+          aux ty1
 let (ty_strictly_positive_in_datacon_decl :
   FStar_TypeChecker_Env.env_t ->
     FStar_Ident.lident Prims.list ->
@@ -739,11 +986,18 @@ let (ty_strictly_positive_in_datacon_decl :
                                          FStar_Parser_Const.binder_strictly_positive_attr in
                                      if uu___4
                                      then
-                                       let uu___5 =
-                                         name_strictly_positive_in_type env
-                                           b.FStar_Syntax_Syntax.binder_bv
-                                           (f.FStar_Syntax_Syntax.binder_bv).FStar_Syntax_Syntax.sort in
-                                       Prims.op_Negation uu___5
+                                       (let uu___5 =
+                                          check_parameter_is_recursively_uniform_in_type
+                                            env mutuals
+                                            b.FStar_Syntax_Syntax.binder_bv
+                                            (f.FStar_Syntax_Syntax.binder_bv).FStar_Syntax_Syntax.sort in
+                                        Prims.op_Negation uu___5) ||
+                                         (let uu___5 =
+                                            name_strictly_positive_in_type
+                                              env
+                                              b.FStar_Syntax_Syntax.binder_bv
+                                              (f.FStar_Syntax_Syntax.binder_bv).FStar_Syntax_Syntax.sort in
+                                          Prims.op_Negation uu___5)
                                      else false) ty_bs1 in
                               match incorrectly_annotated_binder with
                               | FStar_Pervasives_Native.None -> ()
@@ -782,6 +1036,28 @@ let (ty_strictly_positive_in_datacon_decl :
                                            env1 [field] in
                                        check_all_fields env2 fields2))) in
                             check_all_fields env fields))))
+let (open_sig_inductive_typ :
+  FStar_TypeChecker_Env.env ->
+    FStar_Syntax_Syntax.sigelt ->
+      (FStar_TypeChecker_Env.env * (FStar_Ident.lident *
+        FStar_Syntax_Syntax.univ_name Prims.list *
+        FStar_Syntax_Syntax.binders)))
+  =
+  fun env ->
+    fun se ->
+      match se.FStar_Syntax_Syntax.sigel with
+      | FStar_Syntax_Syntax.Sig_inductive_typ
+          (lid, ty_us, ty_params, uu___, uu___1, uu___2) ->
+          let uu___3 = FStar_Syntax_Subst.univ_var_opening ty_us in
+          (match uu___3 with
+           | (ty_usubst, ty_us1) ->
+               let env1 = FStar_TypeChecker_Env.push_univ_vars env ty_us1 in
+               let ty_params1 =
+                 FStar_Syntax_Subst.subst_binders ty_usubst ty_params in
+               let ty_params2 = FStar_Syntax_Subst.open_binders ty_params1 in
+               let env2 = FStar_TypeChecker_Env.push_binders env1 ty_params2 in
+               (env2, (lid, ty_us1, ty_params2)))
+      | uu___ -> failwith "Impossible!"
 let (check_strict_positivity :
   FStar_TypeChecker_Env.env ->
     FStar_Ident.lident Prims.list -> FStar_Syntax_Syntax.sigelt -> Prims.bool)
@@ -790,38 +1066,24 @@ let (check_strict_positivity :
     fun mutuals ->
       fun ty ->
         let unfolded_inductives = FStar_Compiler_Util.mk_ref [] in
-        let uu___ =
-          match ty.FStar_Syntax_Syntax.sigel with
-          | FStar_Syntax_Syntax.Sig_inductive_typ
-              (lid, us, bs, uu___1, uu___2, uu___3) -> (lid, us, bs)
-          | uu___1 -> failwith "Impossible!" in
+        let uu___ = open_sig_inductive_typ env ty in
         match uu___ with
-        | (ty_lid, ty_us, ty_params) ->
+        | (env1, (ty_lid, ty_us, ty_params)) ->
             let mutuals1 = ty_lid :: mutuals in
-            let uu___1 = FStar_Syntax_Subst.univ_var_opening ty_us in
-            (match uu___1 with
-             | (ty_usubst, ty_us1) ->
-                 let env1 = FStar_TypeChecker_Env.push_univ_vars env ty_us1 in
-                 let ty_params1 =
-                   FStar_Syntax_Subst.subst_binders ty_usubst ty_params in
-                 let ty_params2 = FStar_Syntax_Subst.open_binders ty_params1 in
-                 let env2 =
-                   FStar_TypeChecker_Env.push_binders env1 ty_params2 in
-                 let datacons =
-                   let uu___2 =
-                     FStar_TypeChecker_Env.datacons_of_typ env2 ty_lid in
-                   FStar_Pervasives_Native.snd uu___2 in
+            let datacons =
+              let uu___1 = FStar_TypeChecker_Env.datacons_of_typ env1 ty_lid in
+              FStar_Pervasives_Native.snd uu___1 in
+            FStar_Compiler_List.for_all
+              (fun d ->
                  FStar_Compiler_List.for_all
-                   (fun d ->
-                      FStar_Compiler_List.for_all
-                        (fun ty_lid1 ->
-                           let uu___2 =
-                             FStar_Compiler_List.map
-                               (fun uu___3 ->
-                                  FStar_Syntax_Syntax.U_name uu___3) ty_us1 in
-                           ty_strictly_positive_in_datacon_decl env2 mutuals1
-                             ty_lid1 d ty_params2 uu___2 unfolded_inductives)
-                        mutuals1) datacons)
+                   (fun ty_lid1 ->
+                      let uu___1 =
+                        FStar_Compiler_List.map
+                          (fun uu___2 -> FStar_Syntax_Syntax.U_name uu___2)
+                          ty_us in
+                      ty_strictly_positive_in_datacon_decl env1 mutuals1
+                        ty_lid1 d ty_params uu___1 unfolded_inductives)
+                   mutuals1) datacons
 let (check_exn_strict_positivity :
   FStar_TypeChecker_Env.env -> FStar_Ident.lident -> Prims.bool) =
   fun env ->
@@ -829,3 +1091,146 @@ let (check_exn_strict_positivity :
       let unfolded_inductives = FStar_Compiler_Util.mk_ref [] in
       ty_strictly_positive_in_datacon_decl env [] FStar_Parser_Const.exn_lid
         data_ctor_lid [] [] unfolded_inductives
+let (mark_uniform_type_parameters :
+  FStar_TypeChecker_Env.env ->
+    FStar_Syntax_Syntax.sigelt -> FStar_Syntax_Syntax.sigelt)
+  =
+  fun env ->
+    fun sig1 ->
+      let mark_tycon_parameters tc datas =
+        let uu___ = tc.FStar_Syntax_Syntax.sigel in
+        match uu___ with
+        | FStar_Syntax_Syntax.Sig_inductive_typ
+            (tc_lid, us, ty_param_binders, t, mutuals, data_lids) ->
+            let uu___1 = open_sig_inductive_typ env tc in
+            (match uu___1 with
+             | (env1, (tc_lid1, us1, ty_params)) ->
+                 let uu___2 = FStar_Syntax_Util.args_of_binders ty_params in
+                 (match uu___2 with
+                  | (uu___3, ty_param_args) ->
+                      let datacon_fields =
+                        FStar_Compiler_List.filter_map
+                          (fun data ->
+                             match data.FStar_Syntax_Syntax.sigel with
+                             | FStar_Syntax_Syntax.Sig_datacon
+                                 (d_lid, d_us, dt, tc_lid', uu___4, uu___5)
+                                 ->
+                                 let uu___6 =
+                                   FStar_Ident.lid_equals tc_lid1 tc_lid' in
+                                 if uu___6
+                                 then
+                                   let dt1 =
+                                     let uu___7 =
+                                       let uu___8 =
+                                         FStar_Compiler_List.map
+                                           (fun uu___9 ->
+                                              FStar_Syntax_Syntax.U_name
+                                                uu___9) us1 in
+                                       FStar_TypeChecker_Env.mk_univ_subst
+                                         d_us uu___8 in
+                                     FStar_Syntax_Subst.subst uu___7 dt in
+                                   let uu___7 =
+                                     let uu___8 =
+                                       let uu___9 =
+                                         apply_datacon_arrow d_lid dt1
+                                           ty_param_args in
+                                       FStar_Syntax_Util.arrow_formals uu___9 in
+                                     FStar_Pervasives_Native.fst uu___8 in
+                                   FStar_Pervasives_Native.Some uu___7
+                                 else FStar_Pervasives_Native.None
+                             | uu___4 -> FStar_Pervasives_Native.None) datas in
+                      let uniformity_flags =
+                        FStar_Compiler_List.map
+                          (fun ty_param ->
+                             FStar_Compiler_List.for_all
+                               (fun fields_of_one_datacon ->
+                                  FStar_Compiler_List.for_all
+                                    (fun field ->
+                                       check_parameter_is_recursively_uniform_in_type
+                                         env1 mutuals
+                                         ty_param.FStar_Syntax_Syntax.binder_bv
+                                         (field.FStar_Syntax_Syntax.binder_bv).FStar_Syntax_Syntax.sort)
+                                    fields_of_one_datacon) datacon_fields)
+                          ty_params in
+                      let attr =
+                        let fv =
+                          FStar_Syntax_Syntax.lid_as_fv
+                            FStar_Parser_Const.binder_non_uniformly_recursive_parameter_attr
+                            FStar_Syntax_Syntax.delta_constant
+                            FStar_Pervasives_Native.None in
+                        FStar_Syntax_Syntax.fv_to_tm fv in
+                      let uu___4 =
+                        FStar_Compiler_List.fold_left2
+                          (fun uu___5 ->
+                             fun this_param_uniform ->
+                               fun ty_param_binder ->
+                                 match uu___5 with
+                                 | (seen_non_uniform, ty_param_binders1) ->
+                                     if
+                                       seen_non_uniform ||
+                                         (Prims.op_Negation
+                                            this_param_uniform)
+                                     then
+                                       (true,
+                                         ({
+                                            FStar_Syntax_Syntax.binder_bv =
+                                              (ty_param_binder.FStar_Syntax_Syntax.binder_bv);
+                                            FStar_Syntax_Syntax.binder_qual =
+                                              (ty_param_binder.FStar_Syntax_Syntax.binder_qual);
+                                            FStar_Syntax_Syntax.binder_attrs
+                                              = (attr ::
+                                              (ty_param_binder.FStar_Syntax_Syntax.binder_attrs))
+                                          } :: ty_param_binders1))
+                                     else
+                                       (false, (ty_param_binder ::
+                                         ty_param_binders1))) (false, [])
+                          uniformity_flags ty_param_binders in
+                      (match uu___4 with
+                       | (uu___5, ty_param_binders_rev) ->
+                           let ty_param_binders1 =
+                             FStar_Compiler_List.rev ty_param_binders_rev in
+                           let sigel =
+                             FStar_Syntax_Syntax.Sig_inductive_typ
+                               (tc_lid1, us1, ty_param_binders1, t, mutuals,
+                                 data_lids) in
+                           {
+                             FStar_Syntax_Syntax.sigel = sigel;
+                             FStar_Syntax_Syntax.sigrng =
+                               (tc.FStar_Syntax_Syntax.sigrng);
+                             FStar_Syntax_Syntax.sigquals =
+                               (tc.FStar_Syntax_Syntax.sigquals);
+                             FStar_Syntax_Syntax.sigmeta =
+                               (tc.FStar_Syntax_Syntax.sigmeta);
+                             FStar_Syntax_Syntax.sigattrs =
+                               (tc.FStar_Syntax_Syntax.sigattrs);
+                             FStar_Syntax_Syntax.sigopts =
+                               (tc.FStar_Syntax_Syntax.sigopts)
+                           }))) in
+      match sig1.FStar_Syntax_Syntax.sigel with
+      | FStar_Syntax_Syntax.Sig_bundle (ses, lids) ->
+          let uu___ =
+            FStar_Compiler_List.partition
+              (fun se ->
+                 FStar_Syntax_Syntax.uu___is_Sig_inductive_typ
+                   se.FStar_Syntax_Syntax.sigel) ses in
+          (match uu___ with
+           | (tcs, datas) ->
+               let tcs1 =
+                 FStar_Compiler_List.map
+                   (fun tc -> mark_tycon_parameters tc datas) tcs in
+               {
+                 FStar_Syntax_Syntax.sigel =
+                   (FStar_Syntax_Syntax.Sig_bundle
+                      ((FStar_List_Tot_Base.op_At tcs1 datas), lids));
+                 FStar_Syntax_Syntax.sigrng =
+                   (sig1.FStar_Syntax_Syntax.sigrng);
+                 FStar_Syntax_Syntax.sigquals =
+                   (sig1.FStar_Syntax_Syntax.sigquals);
+                 FStar_Syntax_Syntax.sigmeta =
+                   (sig1.FStar_Syntax_Syntax.sigmeta);
+                 FStar_Syntax_Syntax.sigattrs =
+                   (sig1.FStar_Syntax_Syntax.sigattrs);
+                 FStar_Syntax_Syntax.sigopts =
+                   (sig1.FStar_Syntax_Syntax.sigopts)
+               })
+      | uu___ -> sig1
