tests/micro-benchmarks/Positivity.fst
@@ -14,10 +14,7 @@
    limitations under the License.
 *)
 module Positivity
-
 open FStar.All
-
-
 
 type mlist (a:Type) =
   | MNil : mlist a
@@ -27,9 +24,9 @@ and nlist (a:Type) =
   | NNil : nlist a
   | NCons: a -> mlist a -> nlist a
 
-(* this is ok since it's an effectful arrow *)
+(* this is ok since it's an effectful arrow with divergence *)
 noeq type t1 =
-  | C1: (t1 -> ML t1) -> t1
+  | C1: (t1 -> Dv t1) -> t1
 
 (* checking type abbreviations *)
 
@@ -48,8 +45,8 @@ type t =
 
 
 (*
- * #868
- *)
+// //  * #868
+// //  *)
 let l_868: eqtype = (y: Seq.seq int {Seq.mem 2 y })
 type essai_868 = | T of list (l_868 * essai_868)
 
@@ -66,8 +63,8 @@ noeq type t14 =
 
 
 (*
- * Using the strictly_positive attribute on binders
- *)
+// //  * Using the strictly_positive attribute on binders
+// //  *)
 assume val t_t15 (a:Type0) : Type0
 
 [@@ expect_failure]
@@ -89,8 +86,8 @@ type t_t18 =
   | C181: t_t17 t_t18 nat -> t_t18
 
 (*
- * strictly positive attribute is checked properly
- *)
+// //  * strictly positive attribute is checked properly
+// //  *)
 
 val t_t19 ([@@@ strictly_positive] a:Type0) : Type0
 
@@ -101,10 +98,10 @@ let t_t19 a = list a
 
 
 (*
- * This type should be rejected since f may be instantiated with an arrow
- *   that could lead to proof of False, as shown below
- *
- *)
+// //  * This type should be rejected since f may be instantiated with an arrow
+// //  *   that could lead to proof of False, as shown below
+// //  *
+// //  *)
 
 [@@ expect_failure [3]]
 noeq
@@ -129,9 +126,9 @@ let r1 (_:unit) : squash False = g (C201 g)
 
 
 (*
- * If inductive type parameters are marked strictly_positive,
- *   they should be checked properly
- *)
+// //  * If inductive type parameters are marked strictly_positive,
+// //  *   they should be checked properly
+// //  *)
 
 type t_t21 ([@@@ strictly_positive] a:Type0) : Type0 =
   | C211 : a -> t_t21 a
@@ -204,7 +201,7 @@ type sdyn =
   | S : squash (sdyn → GTot ⊥) → sdyn
 
 (* If we don't enforce positivity in refinements,
-   things become inconsistent *)
+// //    things become inconsistent *)
 
 #push-options "--__no_positivity"
 type bad =
@@ -230,3 +227,34 @@ let f (a:Type) (x:a) : option a = Some x
 noeq
 type neg_match =
   | MNM : (match f Type0 neg_match with | Some t -> (t -> bool) | None -> unit) -> neg_match
+
+
+type non_uniform (a:Type) =
+  | NU : non_uniform (a & a) -> non_uniform a
+
+[@@expect_failure [3]]
+type non_uniform_is_not_sp ([@@@strictly_positive]a:Type) =
+  | NUNSP : non_uniform_is_not_sp (a & a) -> non_uniform_is_not_sp a
+
+[@@expect_failure [3]]
+type reject_non_uniform_use =
+  | RNUS : non_uniform reject_non_uniform_use -> reject_non_uniform_use
+
+type mixed_non_uniform (a:Type) (b:Type)  =
+  | MNU : mixed_non_uniform a (b & b) -> mixed_non_uniform a b
+
+type accept_safe_mixed_non_uniform_use =
+  | RNUS : mixed_non_uniform accept_safe_mixed_non_uniform_use unit -> accept_safe_mixed_non_uniform_use
+
+type mixed_non_uniform_prefix (a:Type) (b:Type)  =
+  | MNUP : mixed_non_uniform_prefix (a & a) b -> mixed_non_uniform_prefix a b
+
+[@@expect_failure [3]]
+type reject_safe_mixed_non_uniform_prefix_use =
+  | RNUSP : mixed_non_uniform_prefix unit reject_safe_mixed_non_uniform_prefix_use -> reject_safe_mixed_non_uniform_prefix_use
+
+type flip (a:Type) (b:Type) =
+  | Flip: flip b a -> flip a b
+
+type fail_use_flip =
+  | FUF : flip fail_use_flip bool -> fail_use_flip
